Improvements to the verified LISP interepreters.
The new interpreters have been proved to implement 
McCarthy's LISP 1.5 as formalise by Mike Gordon 
for the ACL2 workshop 2007.

Warning: lisp_evalScript takes 73 minutes to run 
using Holmake under PolyML.

examples/machine-code/compiler/codegenLib.sig
@@ -4,9 +4,9 @@ sig
   include Abbrev
 
   val assemble        : string -> 'a Lib.frag list -> string list
-  val generate_code   : string -> bool -> term -> string list * int
+  val generate_code   : string -> string -> bool -> term -> string list * int
 
-  val add_compiler_assignment : term -> term -> string -> int -> unit
+  val add_compiler_assignment : term -> term -> string -> int -> string -> unit
   val add_compiled            : thm list -> unit
   val print_compiler_grammar  : unit -> unit
 
