examples/machine-code/compiler/codegenLib.sml
@@ -1,8 +1,8 @@
 structure codegenLib :> codegenLib =
 struct
 
-open HolKernel boolLib bossLib Parse;
-open codegen_inputLib helperLib decompilerLib;
+open HolKernel boolLib bossLib Parse decompilerLib;
+open codegen_inputLib helperLib;
 
 (* -- target-specific part begins -- *)
 
@@ -236,18 +236,18 @@ G:      xor eax, 5000`;
 
 (* methods for loading in theorems for use in compilation *)
 
-val compiler_assignments = ref ([]: (term * term * int * string) list);
-val compiler_conditionals = ref ([]: (term * term * int * string) list);
+val compiler_assignments = ref ([]: (term * term * int * string * string) list);
+val compiler_conditionals = ref ([]: (term * term * int * string * string) list);
 
-fun add_compiler_assignment tm1 tm2 name len = 
-  (compiler_assignments := (tm1,tm2,len,name) :: (!compiler_assignments));  
+fun add_compiler_assignment tm1 tm2 name len model_name = 
+  (compiler_assignments := (tm1,tm2,len,name,model_name) :: (!compiler_assignments));  
 
 fun print_compiler_grammar () = let
   val xs = !compiler_assignments
-  fun f (x,y,_,_) = "  let "^(term_to_string x)^" = "^(term_to_string y)^" in _\n"
+  fun f (x,y,_,_,m) = "  " ^ m ^ ":  let "^(term_to_string x)^" = "^(term_to_string y)^" in _\n"
   val assign = map f xs  
   val xs = !compiler_conditionals
-  fun f (x,_,_,_) = "  if "^(term_to_string (repeat dest_neg x))^" then _ else _\n"
+  fun f (x,_,_,_,m) = "  " ^ m ^ ":  if "^(term_to_string (repeat dest_neg x))^" then _ else _\n"
   val cond = map f xs  
   val sorter = sort (curry (fn (x:string,y:string) => x <= y))
   val _ = print "\nAssignments:\n\n"
@@ -257,33 +257,50 @@ fun print_compiler_grammar () = let
   val _ = print "\n"  
   in () end;
 
+fun get_model_name th = let
+  val (m,_,_,_) = (dest_spec o concl o UNDISCH_ALL o SPEC_ALL) th
+  in fst (dest_const m) end;
+
+fun get_tools th = let
+  val s = get_model_name th
+  in if s = "PPC_MODEL" then prog_ppcLib.ppc_tools else
+     if s = "X86_MODEL" then prog_x86Lib.x86_tools else
+     if s = "ARM_MODEL" then prog_armLib.arm_tools else hd [] end
+
 fun add_assignment (tm1,tm2,th,len) = let
+  val (_,_,_,pc) = get_tools th
   val th = RW [GSYM progTheory.SPEC_MOVE_COND] (DISCH_ALL th)
-  val (m,_,_,q) = (dest_spec o concl o SPEC_ALL) th
-  val m = term_to_string m
+  val thx = CONV_RULE (PRE_CONV (SIMP_CONV (std_ss++sep_cond_ss) [])) th
+  val thx = UNDISCH_ALL (RW [progTheory.SPEC_MOVE_COND] thx)
+  val (m,p,_,q) = (dest_spec o concl o SPEC_ALL) thx
+  val m = get_model_name thx
   val name = ("AUTO_"^m^"_ASSIGN_"^(int_to_string (length (!compiler_assignments))))
-  val _ = (compiler_assignments := (tm1,tm2,len,name) :: (!compiler_assignments))
+  val _ = (compiler_assignments := (tm1,tm2,len,name,m) :: (!compiler_assignments))
   val dest_tuple = list_dest pairSyntax.dest_pair
-  val ys = zip (dest_tuple tm1) (dest_tuple tm2) 
+  val ys = zip (dest_tuple tm1) (dest_tuple tm2) handle e => [(tm1,tm2)]
   val ys = filter (fn (x,y) => not (x = y)) ys
-  val q' = subst (map (fn (x,y) => y |-> x) ys) q
+  val post = cdr (find_term (can (match_term (mk_comb(pc,genvar(``:word32``))))) q)
+  val tm2 = subst [mk_var("p",``:word32``) |-> post] p
   val vs = pairSyntax.list_mk_pair (map fst ys)
   val ws = pairSyntax.list_mk_pair (map snd ys)
-  val q' = pairSyntax.mk_anylet([(vs,ws)],q')
-  val th = ONCE_REWRITE_RULE [GSYM (SIMP_CONV std_ss [LET_DEF] q')] th
+  val tm3 = pairSyntax.mk_anylet([(vs,ws)],tm2)
+  val lemma = prove(mk_eq(q,tm3),
+    SPEC_TAC (ws,genvar(type_of ws))
+    THEN SIMP_TAC std_ss [pairTheory.FORALL_PROD,LET_DEF])
+  val th = CONV_RULE (RAND_CONV (ONCE_REWRITE_CONV [lemma])) th
   val _ = add_decompiled (name,th,len,SOME len)
   in () end;
 
 fun add_conditional (tm1,tm2,th,len) = let
   val th = RW [GSYM progTheory.SPEC_MOVE_COND] (DISCH_ALL th)
-  val (m,_,_,_) = (dest_spec o concl o SPEC_ALL) th
-  val m = term_to_string m
+  val m = get_model_name th
   val name = ("AUTO_"^m^"_COND_"^(int_to_string (length (!compiler_conditionals))))
-  val _ = (compiler_conditionals := (tm1,tm2,len,name) :: (!compiler_conditionals))
+  val _ = (compiler_conditionals := (tm1,tm2,len,name,m) :: (!compiler_conditionals))
   val _ = add_decompiled (name,th,len,SOME len)
   in () end;
 
-fun extract_ops tools th = let
+fun extract_ops th = let
+  val tools = (get_tools th)
   val (_,_,th1,pc) = tools
   val (x,y) = dest_eq (concl th1)
   val xs = list_dest dest_star x @ list_dest dest_star y
@@ -312,6 +329,7 @@ fun extract_ops tools th = let
   val tm1 = pairSyntax.list_mk_pair(map fst ys) handle HOL_ERR e => ``()``
   val tm2 = pairSyntax.list_mk_pair(map snd ys) handle HOL_ERR e => ``()``
   val ((tm1,tm2),ys) = if length i = 0 then ((tm1,tm2),ys) else (hd i,i)
+  val len = l
   (* store thm *)
   val _ = if length ys = 0 then () else add_assignment (tm1,tm2,th,l)
   (* possible tests *)
@@ -320,17 +338,7 @@ fun extract_ops tools th = let
   val qs = map (fn tm => add_conditional(foo (cdr tm),car tm,th,l)) qs
   in () end;  
 
-fun add_compiled thms = let
-  fun get_tools th = let
-    val tm = find_term (can (match_term ``SPEC m``)) (concl th)
-    val s = (fst o dest_const o cdr) tm
-    in if s = "PPC_MODEL" then prog_ppcLib.ppc_tools else
-       if s = "X86_MODEL" then prog_x86Lib.x86_tools else
-       if s = "ARM_MODEL" then prog_armLib.arm_tools else hd [] end
-  val _ = map (fn th => extract_ops (get_tools th) th) thms
-  val _ = print_compiler_grammar()
-  in () end;
-
+fun add_compiled thms = let val _ = map extract_ops thms in () end;
 
 (* code generator *)
 
@@ -353,7 +361,7 @@ fun print_asm code = let
         s ^ ":"
   in print "\n\n" ; map (fn s => print (print_inst s ^ "\n")) code ; print "\n\n" end
 
-fun generate_code target print_assembly tm = let
+fun generate_code target model_name print_assembly tm = let
   val (assign2assembly, guard2assembly) = generator_tools target
   val (cond_code, conditionalise, remove_annotations) = conditional_tools target
   (* fold constants *)
@@ -421,12 +429,14 @@ fun generate_code target print_assembly tm = let
   (* ... *)
   (* look up assembly instructions for assignments and comparisions *)
   fun find_assignment (tm1,tm2) [] = hd []
-    | find_assignment (tm1,tm2) ((x,y,l,n)::xs) = 
-        if (tm1 = x) andalso (tm2 = y) then (n,l) else find_assignment (tm1,tm2) xs
+    | find_assignment (tm1,tm2) ((x,y,l,n,m)::xs) = 
+        if (tm1 = x) andalso (tm2 = y) andalso (m = model_name)
+        then (n,l) else find_assignment (tm1,tm2) xs
   fun find_compiled_assignment (tm1,tm2) = find_assignment (tm1,tm2) (!compiler_assignments)
   fun find_conditional tm [] = hd []
-    | find_conditional tm ((x,y,l,n)::xs) = 
-        if (tm = x) orelse (mk_neg tm = x) then (x,y,l,n) else find_conditional tm xs
+    | find_conditional tm ((x,y,l,n,m)::xs) = 
+        if ((tm = x) orelse (mk_neg tm = x)) andalso (m = model_name) 
+        then (x,y,l,n) else find_conditional tm xs
   fun find_compiled_conditional tm = find_conditional tm (!compiler_conditionals)
   fun compile_inst1 (ASM_ASSIGN (t1,t2)) = let
         val (s,i) = find_compiled_assignment (t1,t2) 
