examples/machine-code/compiler/compilerLib.sig
@@ -5,6 +5,7 @@ sig
 
   (* input : target ("arm", "ppc" or "x86") and term (equation defining function) *)
 
-  val compile  : string -> term -> thm * thm * thm
+  val compile      : string -> term -> thm * thm * thm
+  val compile_all  : term -> (string * thm) list * thm * thm
 
 end
