examples/machine-code/compiler/compilerLib.sml
@@ -7,14 +7,31 @@ open prog_armLib prog_ppcLib prog_x86Lib decompilerLib;
 
 open codegenLib helperLib codegen_x86Lib;
 
+val COMPILER_TAC = 
+    SIMP_TAC bool_ss [LET_DEF]
+    THEN REWRITE_TAC [WORD_CMP_NORMALISE] 
+    THEN REWRITE_TAC [WORD_HIGHER,WORD_GREATER,WORD_HIGHER_EQ,
+           WORD_GREATER_EQ,GSYM WORD_NOT_LOWER,GSYM WORD_NOT_LESS] 
+    THEN SIMP_TAC std_ss [WORD_MUL_LSL,word_mul_n2w,word_add_n2w,NOT_IF,
+           WORD_OR_CLAUSES]
+    THEN CONV_TAC (EVAL_ANY_MATCH_CONV word_patterns)
+    THEN SIMP_TAC bool_ss [WORD_SUB_RZERO, WORD_ADD_0, 
+                      AC WORD_ADD_COMM WORD_ADD_ASSOC,
+                      AC WORD_MULT_COMM WORD_MULT_ASSOC,
+                      AC WORD_AND_COMM WORD_AND_ASSOC,
+                      AC WORD_OR_COMM WORD_OR_ASSOC,
+                      AC WORD_XOR_COMM WORD_XOR_ASSOC];
 
+val doing = ref T;
+val target = "arm"
 
 fun compile target tm = let
-  val (tools,target,s) = 
-    if mem target ["arm","ARM"] then (arm_tools,"arm",[]) else 
-    if mem target ["x86","i32","386"] then (x86_tools,"x86",to_x86_regs) else 
-    if mem target ["ppc","Power","PowerPC"] then (ppc_tools,"ppc",[]) else hd []
-  val (code,len) = generate_code target true tm  
+  val _ = (doing := tm)
+  val (tools,target,model_name,s) = 
+    if mem target ["arm","ARM"] then (arm_tools,"arm","ARM_MODEL",[]) else 
+    if mem target ["x86","i32","386"] then (x86_tools,"x86","X86_MODEL",to_x86_regs) else 
+    if mem target ["ppc","Power","PowerPC"] then (ppc_tools,"ppc","PPC_MODEL",[]) else hd []
+  val (code,len) = generate_code target model_name true tm  
   fun append' [] = "" | append' (x::xs) = x ^ "\n" ^ append' xs
   val x = fst (dest_eq tm)
   val name = fst (dest_const (repeat car x)) handle e => fst (dest_var (repeat car x))
@@ -27,34 +44,77 @@ fun compile target tm = let
   val out_tm2 = hd (ends (tm2ftree (cdr tm)))
   val (in_tm,out_tm) = (subst s in_tm, subst s out_tm2)
   val function_in_out = SOME (in_tm,out_tm)
-  val (th1,th2) = basic_decompile tools name function_in_out [QUOTE (append' code)]
-  val const = (repeat car o fst o dest_eq o concl o last o CONJUNCTS) th2
+  val qcode = ([QUOTE (append' code)]) : term Lib.frag list
+  val (th1,th2) = basic_decompile tools name function_in_out qcode
+  val _ = print "Proving equivalence, "
+  val const = (repeat car o fst o dest_eq o concl o hd o CONJUNCTS) th2
   val tm = subst [ repeat car x |-> const ] tm
-  val pre = if is_conj (concl th2) then (hd o CONJUNCTS) th2 else TRUTH
-  val lemma = prove(``(if ~b then x else y) = (if b then y else x:'a)``,Cases_on `b` THEN REWRITE_TAC [])
-(*  
-  set_goal([],tm)
-*)
+  val pre = if is_conj (concl th2) then (last o CONJUNCTS) th2 else TRUTH
   val th3 = prove(tm,
     REPEAT STRIP_TAC
     THEN CONV_TAC (RATOR_CONV (ONCE_REWRITE_CONV [th2]))
-    THEN SIMP_TAC bool_ss [LET_DEF]
-    THEN REWRITE_TAC [WORD_CMP_NORMALISE] 
-    THEN REWRITE_TAC [WORD_HIGHER,WORD_GREATER,WORD_HIGHER_EQ,
-           WORD_GREATER_EQ,GSYM WORD_NOT_LOWER,GSYM WORD_NOT_LESS] 
-    THEN SIMP_TAC std_ss [WORD_MUL_LSL,word_mul_n2w,word_add_n2w,lemma,
-           WORD_OR_CLAUSES]
-    THEN CONV_TAC (EVAL_ANY_MATCH_CONV word_patterns)
-    THEN SIMP_TAC bool_ss [WORD_SUB_RZERO, WORD_ADD_0, 
-                      AC WORD_ADD_COMM WORD_ADD_ASSOC,
-                      AC WORD_MULT_COMM WORD_MULT_ASSOC,
-                      AC WORD_AND_COMM WORD_AND_ASSOC,
-                      AC WORD_OR_COMM WORD_OR_ASSOC,
-                      AC WORD_XOR_COMM WORD_XOR_ASSOC])    
-  val _ = add_compiler_assignment out_tm2 (fst (dest_eq tm)) name len
-  val _ = print (int_to_string len)
+    THEN COMPILER_TAC)    
+  val _ = add_compiler_assignment out_tm2 (fst (dest_eq tm)) name len model_name
+  val _ = print "done.\n"
   in (th1,th3,pre) end
 
+fun compile_all_aux tm = let
+  val x = fst (dest_eq tm)
+  val name = fst (dest_const (repeat car x)) handle e => fst (dest_var (repeat car x))
+  val targets = ["arm","x86","ppc"]
+  fun compile_each tm [] = []
+    | compile_each tm (target::ts) = let
+    val (th,_,_) = compile target tm
+    val base = fetch "-" (name ^ "_base_def")
+    val step = fetch "-" (name ^ "_step_def")
+    val guard = fetch "-" (name ^ "_guard_def")
+    val side = fetch "-" (name ^ "_side_def")
+    val main = fetch "-" (name ^ "")
+    val main_pre = fetch "-" (name ^ "_pre")
+    val def = fetch "-" (name ^ "_def")
+    val pre = fetch "-" (name ^ "_pre_def")
+    val tm = concl def
+    in (target,th,def,pre,[main,main_pre],[base,step,guard,side]) 
+       :: compile_each tm ts end
+  val xs = compile_each tm targets
+  val (_,_,def,pre,tops,parts) = last xs  
+  fun prove_eq (target,th,pre,def,xtops,xparts) = let
+    val f = (repeat car o fst o dest_eq o concl o SPEC_ALL) 
+    val goal = mk_conj(mk_eq(f (hd xtops), f (hd tops)),
+                       mk_eq(f (last xtops), f (last tops)))
+    val lemma = prove(goal,
+      REWRITE_TAC (xtops @ tops)
+      THEN MATCH_MP_TAC tailrecTheory.TAILREC_EQ_THM 
+      THEN REPEAT STRIP_TAC
+      THEN SIMP_TAC std_ss [FUN_EQ_THM,pairTheory.FORALL_PROD]  
+      THEN REWRITE_TAC (xparts @ parts)
+      THEN COMPILER_TAC)  
+    val _ = echo 1 (" " ^ target)
+    in (target, ONCE_REWRITE_RULE [lemma] th) end
+  val _ = echo 1 "\nJoining definitions:"
+  val ys = map prove_eq xs
+  val _ = echo 1 ".\n"
+  val thms = map snd ys
+  val _ = add_compiled (map snd ys)
+  in (ys,def,pre) end; 
 
+fun compile_all tm = let
+  val _ = set_abbreviate_code true
+  fun compile_each [] = []
+    | compile_each (tm::tms) = let
+    val x = car (fst (dest_eq tm))
+    val (ys,def,pre) = compile_all_aux tm    
+    val x2 = (car o fst o dest_eq o concl o SPEC_ALL) def
+    val tms = map (subst [x |-> x2]) tms
+    in (ys,def,pre) :: compile_each tms end
+  val tms = list_dest dest_conj tm
+  val xs = compile_each tms
+  val f = REWRITE_RULE [] o foldr (uncurry CONJ) TRUTH
+  val defs = f (map (fn (x,y,z) => y) xs)
+  val pres = f (map (fn (x,y,z) => z) xs)
+  val (ys,_,_) = last xs 
+  val _ = set_abbreviate_code false
+  val ys = map (fn (n,th) => (n,UNABBREV_CODE_RULE th)) ys  
+  in (ys,defs,pres) end
 
 end;
