examples/machine-code/lisp/lisp_typeScript.sml
@@ -12,7 +12,7 @@ val RW1 = ONCE_REWRITE_RULE;
 
 (* type *)
 
-val _ = Hol_datatype `SExp = Dot of SExp => SExp | Num of num | Sym of string`;
+val _ = Hol_datatype `SExp = Dot of SExp => SExp | Val of num | Sym of string`;
 val SExp_11 = fetch "-" "SExp_11";
 val SExp_distinct = fetch "-" "SExp_distinct";
 
@@ -20,31 +20,42 @@ val SExp_distinct = fetch "-" "SExp_distinct";
 (* definitions *)
 
 val isDot_def = Define `
-  (isDot (Dot x y) = T) /\ (isDot (Num n) = F) /\ (isDot (Sym s) = F)`;
-val isNum_def = Define `
-  (isNum (Dot x y) = F) /\ (isNum (Num n) = T) /\ (isNum (Sym s) = F)`;
+  (isDot (Dot x y) = T) /\ (isDot (Val n) = F) /\ (isDot (Sym s) = F)`;
+val isVal_def = Define `
+  (isVal (Dot x y) = F) /\ (isVal (Val n) = T) /\ (isVal (Sym s) = F)`;
 val isSym_def = Define `
-  (isSym (Dot x y) = F) /\ (isSym (Num n) = F) /\ (isSym (Sym s) = T)`;
+  (isSym (Dot x y) = F) /\ (isSym (Val n) = F) /\ (isSym (Sym s) = T)`;
 
-val getNum_def = Define `
-  (getNum (Dot x y) = 0) /\ (getNum (Num n) = n) /\ (getNum (Sym s) = 0)`;
+val getVal_def = Define `
+  (getVal (Dot x y) = 0) /\ (getVal (Val n) = n) /\ (getVal (Sym s) = 0)`;
 
 val CAR_def = Define `
   (CAR (Dot x y) = x) /\
-  (CAR (Num w) = Num w) /\ 
+  (CAR (Val w) = Val w) /\ 
   (CAR (Sym s) = Sym s)`;
 
 val CDR_def = Define `
   (CDR (Dot x y) = y) /\
-  (CDR (Num w) = Num w) /\ 
+  (CDR (Val w) = Val w) /\ 
   (CDR (Sym s) = Sym s)`;
 
-val LISP_ADD_def   = Define `LISP_ADD  (Num m) (Num n) = Num (m + n)`;
-val LISP_SUB_def   = Define `LISP_SUB  (Num m) (Num n) = Num (m - n)`;
-val LISP_MULT_def  = Define `LISP_MULT (Num m) (Num n) = Num (m * n)`;
-val LISP_DIV_def   = Define `LISP_DIV  (Num m) (Num n) = Num (m DIV n)`;
-val LISP_LESS_def  = Define `LISP_LESS (Num m) (Num n) = m < n`;
-val LISP_EQUAL_def = Define `LISP_EQUAL x y = if x = y then Sym "t" else Sym "nil"`;
+val LISP_ADD_def   = Define `LISP_ADD  (Val m) (Val n) = Val (m + n)`;
+val LISP_SUB_def   = Define `LISP_SUB  (Val m) (Val n) = Val (m - n)`;
+val LISP_MULT_def  = Define `LISP_MULT (Val m) (Val n) = Val (m * n)`;
+val LISP_DIV_def   = Define `LISP_DIV  (Val m) (Val n) = Val (m DIV n)`;
+
+val LISP_TEST_def  = Define `LISP_TEST x = if x then Sym "t" else Sym "nil"`;
+
+val LISP_EQUAL_def   = Define `LISP_EQUAL x y = LISP_TEST (x = y)`;
+val LISP_LESS_def    = Define `LISP_LESS m n  = LISP_TEST (getVal m < getVal n)`;
+val LISP_ATOMP_def   = Define `LISP_ATOMP x   = LISP_TEST (~(isDot x))`;
+val LISP_CONSP_def   = Define `LISP_CONSP x   = LISP_TEST (isDot x)`;
+val LISP_NUMBERP_def = Define `LISP_NUMBERP x = LISP_TEST (isVal x)`;
+val LISP_SYMBOLP_def = Define `LISP_SYMBOLP x = LISP_TEST (isSym x)`;
+
+val TASK_CONT_def = Define `TASK_CONT = Sym "t"`;
+val TASK_EVAL_def = Define `TASK_EVAL = Sym "nil"`;
+val TASK_FUNC_def = Define `TASK_FUNC = Sym "quote"`;
 
 val isQuote_def = Define `
   isQuote x = isDot x /\ (CAR x = Sym "quote") /\ 
@@ -52,12 +63,12 @@ val isQuote_def = Define `
 
 val LSIZE_def = Define `
   (LSIZE (Dot x y) = SUC (LSIZE x + LSIZE y)) /\
-  (LSIZE (Num w) = 0) /\ 
+  (LSIZE (Val w) = 0) /\ 
   (LSIZE (Sym s) = 0)`;
   
 val LDEPTH_def = Define `
   (LDEPTH (Dot x y) = SUC (MAX (LDEPTH x) (LDEPTH y))) /\
-  (LDEPTH (Num w) = 0) /\ 
+  (LDEPTH (Val w) = 0) /\ 
   (LDEPTH (Sym s) = 0)`;
 
 val SUM_LSIZE_def = Define `
@@ -71,9 +82,9 @@ val isDot_thm = store_thm("isDot_thm",
   ``!z. isDot z = ?a b. z = Dot a b``,
   Cases \\ SIMP_TAC std_ss [SExp_11,SExp_distinct,isDot_def]);
 
-val isNum_thm = store_thm("isNum_thm",
-  ``!z. isNum z = ?a. z = Num a``,
-  Cases \\ SIMP_TAC std_ss [SExp_11,SExp_distinct,isNum_def]);
+val isVal_thm = store_thm("isVal_thm",
+  ``!z. isVal z = ?a. z = Val a``,
+  Cases \\ SIMP_TAC std_ss [SExp_11,SExp_distinct,isVal_def]);
 
 val isSym_thm = store_thm("isSym_thm",
   ``!z. isSym z = ?a. z = Sym a``,
