examples/machine-code/lisp/lisp_semanticsScript.sml
@@ -1,0 +1,248 @@
+open HolKernel boolLib bossLib Parse; val _ = new_theory "lisp_semantics";
+
+open stringTheory finite_mapTheory pred_setTheory listTheory sumTheory;
+
+(*****************************************************************************)
+(* Relational semantics for Pure LISP as formalised by Mike Gordon           *)
+(* for the 2006 ACL2 workshop.                                               *)
+(*****************************************************************************)
+
+
+(*****************************************************************************)
+(* An atom is Nil or a number or a string                                    *)
+(*****************************************************************************)
+
+val _ =
+ Hol_datatype
+  `atom = Nil | Number of num | String of string`;
+
+(*****************************************************************************)
+(* An S-expression is an atom or a dotted pair (cons-cell)                   *)
+(*****************************************************************************)
+
+val _ =
+ Hol_datatype
+  `sexpression = A of atom | Cons of sexpression => sexpression`;
+
+(*****************************************************************************)
+(* Syntax of Pure Lisp                                                       *)
+(*****************************************************************************)
+
+val _ =
+ Hol_datatype
+  `term = Con of sexpression
+        | Var of string
+        | App of func => term list
+        | Ite of (term # term)list;
+ 
+   func = FunCon of string
+        | FunVar of string
+        | Lambda of string list => term
+        | Label  of string => func`;
+
+(*****************************************************************************)
+(* Some utility values and functions                                         *)
+(*****************************************************************************)
+
+val False_def =
+ Define
+  `False = A Nil`;
+
+val isTrue_def =
+ Define
+  `isTrue s = ~(s = False) /\ ~(s = A (String "nil"))`;
+
+val True_def =
+ Define
+  `True = A(String "t")`;
+
+val Car_def =
+ Define
+  `Car(Cons s1 s2) = s1`;
+
+val Cdr_def =
+ Define
+  `Cdr(Cons s1 s2) = s2`;
+
+val delete_Nil_aux_def = Define `
+  (delete_Nil_aux Nil = String "nil") /\ 
+  (delete_Nil_aux (Number n) = Number n) /\ 
+  (delete_Nil_aux (String s) = String s)`;
+
+val delete_Nil_def = Define `
+  (delete_Nil (A a) = A (delete_Nil_aux a)) /\ 
+  (delete_Nil (Cons s t) = Cons (delete_Nil s) (delete_Nil t))`;
+
+val Equal_def =
+ Define
+  `Equal (x,y) = if delete_Nil x = delete_Nil y:sexpression then True else False`;
+
+val Atomp_def =
+ Define
+  `(Atomp (A a) = True)
+   /\
+   (Atomp _ = False)`;
+
+val Consp_def =
+ Define
+  `(Consp (A a) = False)
+   /\
+   (Consp _ = True)`;
+
+val Numberp_def =
+ Define
+  `(Numberp (A (Number n)) = True)
+   /\
+   (Numberp _ = False)`;
+
+val Symbolp_def =
+ Define
+  `(Symbolp (A (String s)) = True)
+   /\
+   (Symbolp (A Nil) = True)
+   /\
+   (Symbolp _ = False)`;
+
+val Add_def =
+ Define
+  `Add ((A(Number m)),(A(Number n))) = A(Number(m+n))`;
+
+val Sub_def =
+ Define
+  `Sub ((A(Number m)),(A(Number n))) = A(Number(m-n))`;
+
+val Less_def =
+ Define
+  `Less ((A(Number m)),(A(Number n))) = if m < n then True else False`;
+
+val FunConSem_def =
+ Define
+  `FunConSem s sl =
+    if s = "car"     then Car(EL 0 sl)            else
+    if s = "cdr"     then Cdr(EL 0 sl)            else 
+    if s = "cons"    then Cons(EL 0 sl) (EL 1 sl) else 
+    if s = "+"       then Add(EL 0 sl,EL 1 sl)    else 
+    if s = "-"       then Sub(EL 0 sl,EL 1 sl)    else 
+    if s = "<"       then Less(EL 0 sl,EL 1 sl)   else 
+    if s = "equal"   then Equal(EL 0 sl,EL 1 sl)  else 
+    if s = "atomp"   then Atomp(EL 0 sl)          else 
+    if s = "consp"   then Consp(EL 0 sl)          else 
+    if s = "numberp" then Numberp(EL 0 sl)        else 
+    if s = "symbolp" then Symbolp(EL 0 sl)        else 
+    ARB`;
+
+val FunConSemOK_def =
+ Define
+  `FunConSemOK s sl =
+    if s = "car"     then ?u v. sl = [Cons u v]   else
+    if s = "cdr"     then ?u v. sl = [Cons u v]   else 
+    if s = "cons"    then ?u v. sl = [u; v]       else 
+    if s = "+"       then ?m n. sl = [A (Number m); A (Number n)] else 
+    if s = "-"       then ?m n. sl = [A (Number m); A (Number n)] else 
+    if s = "<"       then ?m n. sl = [A (Number m); A (Number n)] else 
+    if s = "equal"   then ?u v. sl = [u; v]       else 
+    if s = "atomp"   then ?u.   sl = [u]          else 
+    if s = "consp"   then ?u.   sl = [u]          else 
+    if s = "numberp" then ?u.   sl = [u]          else 
+    if s = "symbolp" then ?u.   sl = [u]          else 
+    F`;
+
+(*****************************************************************************)
+(* An environment (alist) is a finite function from names (strings) to       *)
+(* values of type ``:sexpression + func`` (so variables and                  *)
+(* Label-defined functions share the same namespace).                        *)
+(*****************************************************************************)
+
+(*****************************************************************************)
+(* VarBind a xl sl extends a by binding each string in xl to the             *)
+(* S-expression at the corresponding position in sl. If xl is shorter than   *)
+(* sl, then only the first n elements of sl are used, where n is the         *)
+(* length of x. If xl is longer than sl, than sl is padded with NILs.        *)
+(*                                                                           *)
+(* Subtle point: with the semantics in which clock timeout returns NONE      *)
+(* having VarBind  only partially specified is no problem, but               *)
+(* with the semantics in which timeout returns an S-expression it is         *)
+(* tricky to distinguish the arbitrary value returned when VarBind is        *)
+(* applied to lists of different lists from a real value.                    *)
+(* We thus totalise VarBind as described above.                              *)
+(*****************************************************************************)
+
+val VarBind_def =
+ Define
+  `(VarBind a [] sl = (a : (string |-> sexpression + func)))
+   /\
+   (VarBind a (x::xl) [] = (VarBind (a |+ (x, INL(A Nil))) xl []))
+   /\
+   (VarBind a (x::xl) (s::sl) = (VarBind (a |+ (x, INL s)) xl sl))`;
+
+(*****************************************************************************)
+(* 55FunBind a f fn extends a by binding fn to f                               *)
+(*****************************************************************************)
+
+val FunBind_def =
+ Define
+  `FunBind (a:string|->sexpression+func) f fn = a |+ (f, INR fn)`;
+
+(*****************************************************************************)
+(* Operational semantics of Pure Lisp using three inductive relations:       *)
+(*                                                                           *)
+(*  R_ap (fn,args,a) s - fn applied to args evaluates to s with alist a      *)
+(*  R_ev (e,a) s        - term e evaluates to S-expression s with alist a    *)
+(*  R_evl (el,a) sl     - term list el evaluates to S-expression list sl     *)
+(*                                                                           *)
+(* The names R_evl_rules, R_evl_ind, R_evl_cases are the ones                *)
+(* automatically generated to name the theorems in the theory.               *)
+(*                                                                           *)
+(*****************************************************************************)
+
+val (R_ap_rules,R_ap_ind,R_ap_cases) =
+ Hol_reln
+ `(!s a. 
+    R_ev (Con s, a) s)
+  /\
+  (!x a. 
+    x IN FDOM a /\ ISL (a ' x) ==> 
+    R_ev (Var x, a) (OUTL(a ' x)))
+  /\
+  (!fc args a.
+    FunConSemOK fc args ==>
+    R_ap (FunCon fc,args,a) (FunConSem fc args))
+  /\
+  (!fn el args s a. 
+    R_evl (el,a) args /\ R_ap (fn,args,a) s /\ (LENGTH args = LENGTH el)
+    ==> R_ev (App fn el,a) s)
+  /\
+  (!a.
+    R_ev (Ite [], a) False)
+  /\
+  (!e1 e2 el s a. 
+    R_ev (e1,a) False /\ R_ev (Ite el,a) s
+    ==> R_ev (Ite ((e1,e2)::el),a) s)
+  /\
+  (!e1 e2 el s1 s a.
+    R_ev (e1,a) s1 /\ isTrue s1 /\ R_ev (e2,a) s 
+    ==>
+    R_ev (Ite ((e1,e2)::el),a) s)
+  /\
+  (!x fn args s a. 
+    R_ap (fn,args,FunBind a x fn) s ==> R_ap(Label x fn,args,a) s)
+  /\
+  (!fv args s a.
+    fv NOTIN {"quote";"cond";"car";"cdr";"cons";"+";"-";"<";
+              "equal";"atomp";"consp";"symbolp";"numberp"} /\
+    fv IN FDOM a /\ ISR (a ' fv) /\ 
+    R_ap (OUTR(a ' fv),args,a) s ==> R_ap (FunVar fv,args,a) s)
+  /\
+  (!xl e args s a.
+    (LENGTH args = LENGTH xl) /\ R_ev (e,VarBind a xl args) s 
+    ==> R_ap (Lambda xl e,args,a) s)
+  /\
+  (!a.
+    R_evl ([],a) [])
+  /\
+  (!e el s sl a.
+    R_ev (e,a) s /\ R_evl (el,a) sl
+    ==> R_evl (e::el,a) (s::sl))`;
+
+val _ = export_theory();
+
